.

src/program_proof/session/u64ToNat.v
@@ -1,9 +1,106 @@
 Require Import Perennial.program_proof.session.session_definitions.
 
+Reserved Infix ">>=" (left associativity, at level 90).
 Reserved Infix "=~=" (at level 70, no associativity).
+
+(** Section MONAD. *)
+
+#[universes(polymorphic=yes)]
+Class isMonad@{d c} (M : Type@{d} -> Type@{c}) : Type :=
+  { bind {A : Type@{d}} {B : Type@{d}} (m : M A) (k : A -> M B) : M B
+  ; pure {A : Type@{d}} : A -> M A
+  }.
+
+Infix ">>=" := bind.
+
+#[universes(polymorphic=yes)]
+Definition monad@{u v} {M : Type@{u} -> Type@{v}} {MONAD : isMonad@{u v} M} {A : Type@{u}} : Type@{v} :=
+  M A.
+
+Declare Scope monad_scope.
+Declare Custom Entry do_notation.
+
+Delimit Scope monad_scope with monad.
+Bind Scope monad_scope with monad.
+Open Scope monad_scope.
+
+Reserved Notation "'do' m" (m custom do_notation at level 10, at level 0, format "'do'  '//' m").
+Notation "'do' m" := m : monad_scope.
+Notation "'do' m" := (m : monad).
+
+Notation "x '<-' m1 ';' m2" := (m1 >>= fun x => m2) (in custom do_notation at level 0, x ident, m1 constr, m2 custom do_notation at level 10, format "x  '<-'  m1 ';' '//' m2").
+Notation "'let' x ':=' t ';' m" := (let x := t in m) (in custom do_notation at level 0, x pattern, t constr, m custom do_notation at level 10, format "'let'  x  ':='  t ';' '//' m").
+Notation "''' x '<-' m1 ';' m2" := (m1 >>= fun 'x => m2) (in custom do_notation at level 0, x pattern, m1 constr, m2 custom do_notation at level 10, format "''' x  '<-'  m1 ';' '//' m2").
+Notation "m1 ';' m2" := (m1 >>= fun _ => m2) (in custom do_notation at level 0, m1 constr, m2 custom do_notation at level 10, format "m1 ';' '//' m2").
+Notation "'ret' t" := (pure t) (in custom do_notation at level 10, t constr, format "'ret'  t").
+Notation "t" := t (in custom do_notation at level 0, t constr).
+
+#[global]
+Instance option_isMonad : isMonad option :=
+  { pure {A} := @Some A
+  ; bind {A} {B} (m : option A) (k : A -> option B) :=
+    match m with
+    | Some x => k x
+    | None => None
+    end
+  }.
+
+(** End MONAD. *)
+
+(** Section OPTION. *)
+
+Fixpoint fold_left_option {A : Type} {B : Type} (f : A -> B -> option A) (xs : list B) (z : A) : option A :=
+  match xs with
+  | [] => do
+    ret z
+  | x :: xs' => do
+    'y <- f z x;
+    fold_left_option f xs' y
+  end.
+
+(** End OPTION. *)
+
+(** Section SIMILARITY. *)
 
 #[universes(template)]
 Class Similarity (A : Type) (A' : Type) : Type :=
   is_similar_to (x : A) (x' : A') : Prop.
 
 Infix "=~=" := is_similar_to.
+
+Inductive list_corres {A : Type} {A' : Type} {SIM : Similarity A A'} : Similarity (list A) (list A') :=
+  | nil_corres
+    : [] =~= []
+  | cons_corres (x : A) (x' : A') (xs : list A) (xs' : list A')
+    (head_corres : x =~= x')
+    (tail_corres : xs =~= xs')
+    : x :: xs =~= x' :: xs'.
+
+#[local] Hint Constructors list_corres : core.
+
+#[global]
+Instance Similarity_list {A : Type} {A' : Type} (SIM : Similarity A A') : Similarity (list A) (list A') :=
+  @list_corres A A' SIM.
+
+(** End SIMILARITY. *)
+
+(** Section BASIC_CORRES. *)
+
+Definition param2func_corres {A : Type} {A' : Type} {B : Type} {B' : Type} {C : Type} {C' : Type} `{Similarity A A'} `{Similarity B B'} `{Similarity C C'} (f : A -> B -> C) (f' : A' -> B' -> option C') : Prop :=
+  forall a' : A', forall b' : B', forall c' : C', f' a' b' = Some c' ->
+  forall a : A, a =~= a' ->
+  forall b : B, b =~= b' ->
+  exists c : C, c =~= c' /\ f a b = c.
+
+Lemma fold_left_option_corres `{Similarity A A'} `{Similarity B B'} (f : A -> B -> A) (f' : A' -> B' -> option A')
+  (f_corres : param2func_corres f f')
+  : param2func_corres (fold_left f) (fold_left_option f').
+Proof.
+  red. intros xs' z' y' H_OBS xs xs_corres z z_corres. revert z z' y' z_corres H_OBS.
+  induction xs_corres as [ | x x' xs xs' x_corres xs_corres IH]; simpl; intros.
+  - exists z. split; ss!.
+  - destruct (f' z' x') as [_y' | ] eqn: H_y'; try congruence. eapply IH with (z' := _y'); trivial.
+    pose proof (f_corres z' x' _y' H_y' z z_corres x x_corres) as (? & H_y & <-); trivial.
+Qed.
+
+(** End BASIC_CORRES. *)
